pulse/share/steel/examples/pulse/dice/X509.fst
@@ -1,0 +1,81 @@
+module X509
+module R = Steel.ST.Reference
+module A = Steel.ST.Array
+module T = FStar.Tactics
+module PM = Pulse.Main
+open Steel.ST.Util 
+open Steel.ST.Array
+open Steel.FractionalPermission
+open FStar.Ghost
+open Pulse.Steel.Wrapper
+module A = Steel.ST.Array
+module US = FStar.SizeT
+module U8 = FStar.UInt8
+module U32 = FStar.UInt32
+open HACL
+open L0Types
+open L0Crypto
+
+assume
+val length_of_deviceIDCSR (len: U32.t) : U32.t 
+
+assume
+val len_of_deviceIDCRI
+  (version: U32.t)
+  (s_common: string)
+  (s_org: string)
+  (s_country: string)
+  : U32.t
+
+assume
+val serialize_deviceIDCSR 
+  (deviceIDCRI_len: U32.t)
+  (deviceIDCSR: deviceIDCSR_t deviceIDCRI_len)
+  : Seq.seq U8.t
+
+assume
+val spec_serialize_deviceIDCRI
+  (deviceIDCRI: deviceIDCRI_t)
+  : Seq.seq U8.t
+
+assume
+val serialize_deviceIDCRI
+  (deviceIDCRI: deviceIDCRI_t)
+  (deviceIDCRI_len: U32.t)
+  (deviceIDCRI_buf: A.array U8.t)
+  (#deviceIDCRI_buf0: Ghost.erased (Seq.seq U8.t))
+  : stt unit
+    (A.pts_to deviceIDCRI_buf full_perm deviceIDCRI_buf0)
+    (fun _ -> A.pts_to deviceIDCRI_buf full_perm (spec_serialize_deviceIDCRI deviceIDCRI))
+
+assume 
+val spec_x509_get_deviceIDCRI
+  (version: U32.t)
+  (s_common: string)
+  (s_org: string)
+  (s_country: string)
+  (ku: U32.t)
+  (deviceID_pub: Seq.seq U8.t)
+  : deviceIDCRI_t
+
+assume 
+val x509_get_deviceIDCRI
+  (version: U32.t)
+  (s_common: string)
+  (s_org: string)
+  (s_country: string)
+  (ku: U32.t)
+  (deviceID_pub: A.array U8.t)
+  (#deviceID_pub0: Ghost.erased (Seq.seq U8.t))
+  : stt deviceIDCRI_t
+    (A.pts_to deviceID_pub full_perm deviceID_pub0)
+    (fun res -> 
+      A.pts_to deviceID_pub full_perm deviceID_pub0 `star`
+      pure (res == spec_x509_get_deviceIDCRI version s_common s_org s_country ku deviceID_pub0))
+
+assume
+val serialize32_deviceIDCRI_backwards
+  (deviceIDCRI: deviceIDCRI_t)
+  (deviceIDCRI_len: U32.t)
+  (deviceIDCRI_buf: A.array U8.t)
+  : U32.t
